ulib/FStar.HyperHeap.fst
@@ -229,7 +229,14 @@ abstract val lemma_disjoint_parents: pr:rid -> r:rid -> ps:rid -> s:rid -> Lemma
 let lemma_disjoint_parents pr r ps s = ()
 
 let contains_ref (#a:Type) (#i:rid) (r:rref i a) (m:t) : GTot bool =
-    Map.contains m i && Heap.contains (Map.sel m i) (as_ref r)
+  Map.contains m i && Heap.contains (Map.sel m i) (as_ref r)
+
+(*
+ * AR: using this from HyperStack:weak_contains,
+ * Map.contains covered by weak_live_region in HyperStack
+ *)
+let weak_contains_ref (#a:Type) (#i:rid) (r:rref i a) (m:t) : GTot bool =
+  Heap.contains (Map.sel m i) (as_ref r)
 
 let fresh_rref (#a:Type) (#i:rid) (r:rref i a) (m0:t) (m1:t) =
   not (Heap.contains (Map.sel m0 i) (as_ref r))
