ulib/hyperstack/FStar.ST.fst
@@ -144,6 +144,14 @@ let fresh_region (r:HH.rid) (m0:mem) (m1:mem) =
   not (r `is_in` m0.h)
   /\ r `is_in` m1.h
 
+(*
+ * AR: using this in mitls code, so that it corresponds to the
+ * fresh_region definition in hyperheap.
+ *)
+let stronger_fresh_region (r:HH.rid) (m0:mem) (m1:mem) =
+   (forall j. HH.includes r j ==> not (j `is_in` m0.h))
+   /\ r `is_in` m1.h
+
 assume val new_region: r0:HH.rid -> ST HH.rid
       (requires (fun m -> is_eternal_region r0))
       (ensures (fun (m0:mem) (r1:HH.rid) (m1:mem) ->
@@ -203,8 +211,11 @@ inline let deref_post (#a:Type) (r:reference a) m0 x m1 =
    Dereferences, provided that the reference exists.
    Guaranties the strongest low-level effect: Stack
    *)
+(*
+ * AR: making the precondition as weak_contains.
+ *)
 assume val op_Bang: #a:Type -> r:reference a -> Stack a
-  (requires (fun m -> m `contains` r))
+  (requires (fun m -> m `weak_contains` r))
   (ensures (deref_post r))
 
 let modifies_none (h0:mem) (h1:mem) = modifies Set.empty h0 h1
